src/AtomicSteps.v
@@ -84,15 +84,15 @@ Section AtomicSteps.
       AtomicSteps stepCondTop ioss soss (rqImpl :: nil) ->
       ioss ≈ soss ->
       forall ist1 sst1,
-        tst_oss ist1 = ioss ->
-        tst_oss sst1 = soss ->
+        st_oss ist1 = ioss ->
+        st_oss sst1 = soss ->
         forall ihst ist2 mouts,
           steps_det impl ist1 ihst ist2 ->
-          Atomic impl trsIdx (toTMsgU rqImpl) ihst mouts ->
+          Atomic impl rqImpl ihst mouts ->
           exists sst2 shst,
             steps_det spec sst1 shst sst2 /\
             map p (behaviorOf impl ihst) = behaviorOf spec shst /\
-            tst_oss ist2 ≈ tst_oss sst2.
+            st_oss ist2 ≈ st_oss sst2.
   Proof.
   Admitted.
 
