src/StepDet.v
@@ -1,70 +1,38 @@
 Require Import Bool List String Peano_dec.
 Require Import Common FMap Syntax Semantics.
 
-Inductive step_det (sys: System) : TState -> TLabel -> TState -> Prop :=
+Inductive step_det (sys: System) : MState -> MLabel -> MState -> Prop :=
 | SdSlt: forall st, step_det sys st emptyILabel st
-| SdExt: forall ts oss oims emsg,
+| SdExt: forall oss oims emsg,
     isExternal sys (mid_from (msg_id emsg)) = true ->
     isInternal sys (mid_to (msg_id emsg)) = true ->
     step_det sys
-             {| tst_oss := oss; tst_msgs := oims; tst_tid := ts |}
-             (IlblIn (toTMsgU emsg))
-             {| tst_oss := oss;
-                tst_msgs := distributeMsg (toTMsgU emsg) oims;
-                tst_tid := ts
-             |}
-| SdIntInit: forall ts nts (Hts: nts > ts) oss oims obj oidx os pos
-                    (fmsg: TMsg) fpmsg fidx fchn outs,
+             {| st_oss := oss; st_msgs := oims |}
+             (IlblIn emsg)
+             {| st_oss := oss; st_msgs := distributeMsg emsg oims |}
+| SdInt: forall oss oims obj oidx os pos fmsg fpmsg fidx fchn outs,
     In obj (sys_objs sys) ->
     oidx = obj_idx obj ->
     (oss)@[oidx] = Some os ->
 
-    isExternal sys (mid_from (msg_id (getMsg fmsg))) = true ->
-    tmsg_tid fmsg = None ->
+    isExternal sys (mid_from (msg_id fmsg)) = true ->
 
     ValidMsgId fidx oidx fchn fmsg ->
     firstM fidx oidx fchn oims = Some fmsg -> 
 
-    msg_id (getMsg fmsg) = pmsg_mid fpmsg ->
+    msg_id fmsg = pmsg_mid fpmsg ->
     In fpmsg (obj_trs obj) ->
     pmsg_precond fpmsg os ->
-    pmsg_postcond fpmsg os (msg_value (getMsg fmsg)) pos ->
-    outs = pmsg_outs fpmsg os (msg_value (getMsg fmsg)) ->
+    pmsg_postcond fpmsg os (msg_value fmsg) pos ->
+    outs = pmsg_outs fpmsg os (msg_value fmsg) ->
     ValidOuts oidx outs ->
 
     step_det sys
-             {| tst_oss := oss; tst_msgs := oims; tst_tid := ts |}
-             (IlblOuts (Some (toTMsg nts (getMsg fmsg))) (toTMsgs nts outs))
-             {| tst_oss := oss +[ oidx <- pos ];
-                tst_msgs := distributeMsgs (intOuts sys (toTMsgs nts outs)) oims;
-                tst_tid := nts
-             |}
-| SdIntFwd: forall ts mts oss oims obj oidx os pos
-                   (fmsg: TMsg) fpmsg fidx fchn outs,
-    In obj (sys_objs sys) ->
-    oidx = obj_idx obj ->
-    (oss)@[oidx] = Some os ->
-
-    isInternal sys (mid_from (msg_id (getMsg fmsg))) = true ->
-    tmsg_tid fmsg = Some mts ->
-
-    ValidMsgId fidx oidx fchn fmsg ->
-    firstM fidx oidx fchn oims = Some fmsg -> 
-
-    msg_id (getMsg fmsg) = pmsg_mid fpmsg ->
-    In fpmsg (obj_trs obj) ->
-    pmsg_precond fpmsg os ->
-    pmsg_postcond fpmsg os (msg_value (getMsg fmsg)) pos ->
-    outs = pmsg_outs fpmsg os (msg_value (getMsg fmsg)) ->
-    ValidOuts oidx outs ->
-
-    step_det sys
-             {| tst_oss := oss; tst_msgs := oims; tst_tid := ts |}
-             (IlblOuts (Some fmsg) (toTMsgs mts outs))
-             {| tst_oss := oss +[ oidx <- pos ];
-                tst_msgs := distributeMsgs (intOuts sys (toTMsgs mts outs)) oims;
-                tst_tid := ts
+             {| st_oss := oss; st_msgs := oims |}
+             (IlblOuts (Some fmsg) outs)
+             {| st_oss := oss +[ oidx <- pos ];
+                st_msgs := distributeMsgs (intOuts sys outs) oims
              |}.
 
-Definition steps_det: Steps TState TLabel := steps step_det.
+Definition steps_det: Steps MState MLabel := steps step_det.
 
